theories/binary_format_spec.v
@@ -1,14 +1,14 @@
 From Wasm Require Import datatypes_properties binary_format_parser binary_format_printer.
 From compcert Require Import Integers.
 From parseque Require Import Parseque.
-Require Import Ascii Byte.
+Require Import Byte.
 Require Import leb128.
 Require Import Coq.Arith.Le.
 
-Inductive repr_unsigned : list ascii -> module -> Prop :=
+Inductive repr_unsigned : list byte -> module -> Prop :=
 .
 
-Inductive repr_module : list ascii -> module -> Prop :=
+Inductive repr_module : list byte -> module -> Prop :=
 .
 
 (* TODO: we should have ast->binary->ast = id
@@ -16,6 +16,6 @@ Inductive repr_module : list ascii -> module -> Prop :=
 
 Lemma encode_decode_is_identity : forall m,
 (* TODO: probably need some well-formedness condition, for example of block types *)
-  run_parse_module_from_bytes (binary_of_module m) = Some m.
+  run_parse_module (binary_of_module m) = Some m.
 (* TODO *)
 Admitted.
