theories/check_toks.v
@@ -5,13 +5,13 @@ Require Import Coq.Arith.Le.
 Section Check.
 
 Context
-  {Toks : nat -> Type} `{Sized Toks Ascii.ascii}
+  {Toks : nat -> Type} `{Sized Toks Byte.byte}
   {M : Type -> Type} `{RawMonad M} `{RawAlternative M} `{RawMonadRun M}
   {Tok : Type} `{Tokenizer Tok}
   {A : Type}.
 
-Definition check_toks : list Byte.byte -> [ Parser (SizedList Ascii.ascii) Ascii.ascii M A ] -> Type := fun s p =>
-  let tokens := List.map Ascii.ascii_of_byte s in
+Definition check_toks : list Byte.byte -> [ Parser (SizedList Byte.byte) Byte.byte M A ] -> Type := fun s p =>
+  let tokens := s in
   let n      := List.length tokens in
   let input  := mkSizedList tokens in
   let result := runParser (p n) (le_refl n) input in
